offsets_and_sizes_are_contiguous, sorted

src/Parquet/Parquet.Spec.Jump.fst
@@ -36,3 +36,53 @@ let jump_with_offset_and_size_then_parse
     else
       let new_b = Seq.slice b offset (offset + size) in
       coerce_ (parse (parse_fldata' p size) new_b)
+
+let rec offsets_and_sizes_are_contiguous
+  (l: list (nat & nat))
+: Tot bool
+= match l with
+  | (off1, sz1) :: (off2, sz2) :: q ->
+    off1 + sz1 = off2 &&
+    offsets_and_sizes_are_contiguous ((off2, sz2) :: q)
+  | _ -> true
+
+let rec offsets_and_sizes_are_sorted
+  (l: list (nat & nat))
+: Tot bool
+= match l with
+  | (off1, sz1) :: (off2, sz2) :: q ->
+    off1 + sz1 <= off2 &&
+    offsets_and_sizes_are_sorted ((off2, sz2) :: q)
+  | _ -> true
+
+let rec offsets_and_sizes_are_contiguous_implies_sorted
+  (l: list (nat & nat))
+: Lemma
+  (requires (offsets_and_sizes_are_contiguous l))
+  (ensures (offsets_and_sizes_are_sorted l))
+= match l with
+  | (off1, sz1) :: (off2, sz2) :: q ->
+    offsets_and_sizes_are_contiguous_implies_sorted ((off2, sz2) :: q)
+  | _ -> ()
+
+let rec offsets_and_sizes_are_sorted_disjoint
+  (l: list (nat & nat))
+  (i1 i2: nat)
+: Lemma
+  (requires (
+    offsets_and_sizes_are_sorted l /\
+    i1 < i2 /\
+    i2 < List.Tot.length l
+  ))
+  (ensures (
+    let (off1, sz1) = List.Tot.index l i1 in
+    let (off2, _) = List.Tot.index l i2 in
+    off1 + sz1 <= off2
+  ))
+  (decreases (List.Tot.length l))
+= if i1 = 0 then begin
+    let (off1, sz1) :: (off15, sz15) :: q = l in
+    if i2 = 1 then () else 
+    offsets_and_sizes_are_sorted_disjoint ((off1, off15 - off1 + sz15) :: q) 0 (i2 - 1)
+  end
+  else offsets_and_sizes_are_sorted_disjoint (List.Tot.tl l) (i1 - 1) (i2 - 1)
